tuned and example

Network_Security_Policy_Verification/SINVAR_Examples.thy
@@ -15,9 +15,31 @@ definition make_policy :: "('a SecurityInvariant) list \<Rightarrow> 'a list \<R
   "make_policy sinvars V \<equiv> generate_valid_topology sinvars \<lparr>nodesL = V, edgesL = List.product V V \<rparr>"
 
 
-definition exampleG :: "nat list_graph" where
-  "exampleG \<equiv> \<lparr> nodesL = [1, 2, 3],
-                edgesL = [(1,2), (2,3)]\<rparr>"
+abbreviation "V\<equiv>TopoS_Vertices.V"
+
+context begin
+  private definition "ACL_m \<equiv> new_configured_list_SecurityInvariant SINVAR_LIB_CommunicationPartners \<lparr> 
+          node_properties = [V ''db1'' \<mapsto> Master [V ''h1'', V ''h2''],
+                             V ''db2'' \<mapsto> Master [V ''db1''],
+                             V ''h1'' \<mapsto> Care,
+                             V ''h2'' \<mapsto> Care
+                             ], 
+          model_global_properties = () 
+          \<rparr>" 
+  value[code] "make_policy [ACL_m] [V ''db1'', V ''db2'', V ''h1'', V ''h2'', V ''h3'']"
+  ML_val{*
+  visualize_graph_header @{context} @{term "[ACL_m]"}
+    @{term "make_policy [ACL_m] [V ''db1'', V ''db2'', V ''h1'', V ''h2'', V ''h3'']"}
+    @{term "[V ''db1'' \<mapsto> Master [V ''h1'', V ''h2''],
+             V ''db2'' \<mapsto> Master [V ''db1''],
+             V ''h1'' \<mapsto> Care,
+             V ''h2'' \<mapsto> Care
+             ]"};
+  *}
+end
+
+
+
 
 definition CommWith_m::"(nat SecurityInvariant)" where
     "CommWith_m \<equiv> new_configured_list_SecurityInvariant SINVAR_LIB_ACLcommunicateWith \<lparr> 
@@ -30,7 +52,9 @@ definition CommWith_m::"(nat SecurityInvariant)" where
 
 text{*Experimental: the config (only one) can be added to the end.*}
 ML_val{*
-visualize_graph_header @{context} @{term "[CommWith_m]"} @{term "exampleG"} @{term "[
+visualize_graph_header @{context} @{term "[CommWith_m]"}
+       @{term "\<lparr> nodesL = [1::nat, 2, 3],
+                edgesL = [(1,2), (2,3)]\<rparr>"} @{term "[
                   (1::nat) \<mapsto> [2::nat,3],
                   2 \<mapsto> [3]]"};
 *}
@@ -50,3 +74,61 @@ visualize_graph @{context} @{term "[ new_configured_list_SecurityInvariant SINVA
           model_global_properties = () 
           \<rparr>]"} @{term "\<lparr>nodesL = [1::nat,2,3,4], edgesL = [(1,2), (1,3), (2,3), (3, 4)] \<rparr>"};
 *}
+
+
+
+context begin
+  private definition G_dep :: "nat list_graph" where
+    "G_dep \<equiv> \<lparr>nodesL = [1::nat,2,3,4,5,6,7], edgesL = [(1,2), (2,1), (2,3),
+                                                       (4,5), (5,6), (6,7)] \<rparr>"
+  private lemma "wf_list_graph G_dep" by eval
+
+  private definition "DEP_m \<equiv> new_configured_list_SecurityInvariant SINVAR_LIB_Dependability \<lparr> 
+          node_properties = Some \<circ> dependability_fix_nP G_dep (\<lambda>_. 0),
+          model_global_properties = () 
+          \<rparr>"
+  ML_val{* 
+  visualize_graph_header @{context} @{term "[DEP_m]"}
+    @{term "G_dep"}
+    @{term "Some \<circ> dependability_fix_nP G_dep (\<lambda>_. 0)"};
+  *}
+
+  text{*Connecting @{term "(3,4)"}. This causes only one offedning flow at @{term "(3,4)"}.*}
+  ML_val{*
+  visualize_graph_header @{context} @{term "[DEP_m]"}
+    @{term "G_dep\<lparr>edgesL := (3,4)#edgesL G_dep\<rparr>"}
+    @{term "Some \<circ> dependability_fix_nP G_dep (\<lambda>_. 0)"};
+  *}
+  text{*We try to increase the dependability level at @{term 3}. Suddenly, offending flows everywhere.*}
+  ML_val{*
+  visualize_graph_header @{context} @{term "[new_configured_list_SecurityInvariant SINVAR_LIB_Dependability \<lparr> 
+          node_properties = Some \<circ> ((dependability_fix_nP G_dep (\<lambda>_. 0))(3 := 2)),
+          model_global_properties = () 
+          \<rparr>]"}
+    @{term "G_dep\<lparr>edgesL := (3,4)#edgesL G_dep\<rparr>"}
+    @{term "Some \<circ> ((dependability_fix_nP G_dep (\<lambda>_. 0))(3 := 2))"};
+  *}
+  lemma "implc_offending_flows (new_configured_list_SecurityInvariant SINVAR_LIB_Dependability \<lparr> 
+                          node_properties = Some \<circ> ((dependability_fix_nP G_dep (\<lambda>_. 0))(3 := 2)),
+                          model_global_properties = () 
+                          \<rparr>)
+             (G_dep\<lparr>edgesL := (3,4)#edgesL G_dep\<rparr>) = 
+           [[(3, 4)], [(1, 2), (2, 1), (5, 6)], [(1, 2), (4, 5)], [(2, 1), (4, 5)], [(2, 3), (4, 5)], [(2, 3), (5, 6)]]"
+           by eval
+
+  text{*If we recompute the dependability levels for the changed graph, we see that suddenly, 
+        The level at @{term 1} and @{term 2} increased, though we only added the edge @{term "(3,4)"}.
+        This hints that we connected the graph. If an attacker can now compromise @{term 1}, she 
+        may be able to peek much deeper into the network.*}
+  ML_val{*
+  visualize_graph_header @{context} @{term "[new_configured_list_SecurityInvariant SINVAR_LIB_Dependability \<lparr> 
+          node_properties = Some \<circ> dependability_fix_nP (G_dep\<lparr>edgesL := (3,4)#edgesL G_dep\<rparr>) (\<lambda>_. 0),
+          model_global_properties = () 
+          \<rparr>]"}
+    @{term "G_dep\<lparr>edgesL := (3,4)#edgesL G_dep\<rparr>"}
+    @{term "Some \<circ> dependability_fix_nP (G_dep\<lparr>edgesL := (3,4)#edgesL G_dep\<rparr>) (\<lambda>_. 0)"};
+  *}
+
+end
+
+
